Moist.lean
@@ -18,5 +18,5 @@ import Moist.Plutus.PrettyHuman
 import Moist.Plutus.Eval
 import Moist.Onchain
 import Moist.SMT.Semantics
-import Moist.SMT.UPLC
+import Moist.SMT.Compiler
 import Moist.SMT.Soundness
